Prove w8array_substring_spec

characteristic/cfScript.sml
@@ -1325,6 +1325,16 @@ val app_copystraw8_def = Define `
             ==>> Q (Val (Conv NONE [])))) /\
      Q ==e> POST_F)`
 
+val app_copyaw8str_def = Define `
+  app_copyaw8str s so l H Q =
+    ((?ws F.
+        0 <= so /\ 0 <= l /\
+        (Num so + Num l) <= LENGTH ws /\
+        (H ==>> F * W8ARRAY s ws) /\
+        (F * W8ARRAY s ws
+            ==>> Q (Val (Litv (StrLit (MAP (CHR o w2n) (TAKE (Num l) (DROP (Num so) ws)))))))) /\
+     Q ==e> POST_F)`
+
 val app_wordFromInt_W8_def = Define `
   app_wordFromInt_W8 (i: int) H Q =
     (H ==>> Q (Val (Litv (Word8 (i2w i)))) /\
@@ -1556,6 +1566,14 @@ val cf_copystraw8_def = Define `
       exp2v env xdo = SOME (Litv (IntLit do)) /\
       app_copystraw8 s so l d do H Q)`
 
+val cf_copyaw8str_def = Define `
+  cf_copyaw8str xs xso xl = \env. local (\H Q.
+    ?s so l.
+      exp2v env xs = SOME s /\
+      exp2v env xso = SOME (Litv (IntLit so)) /\
+      exp2v env xl = SOME (Litv (IntLit l)) /\
+      app_copyaw8str s so l H Q)`
+
 val cf_wordFromInt_W8_def = Define `
   cf_wordFromInt_W8 xi = \env. local (\H Q.
     ?i.
@@ -1725,6 +1743,10 @@ val cf_def = tDefine "cf" `
           (case args of
              | [s; so; l; d; do] => cf_copystraw8 s so l d do
              | _ => cf_bottom)
+        | CopyAw8Str =>
+          (case args of
+             | [s; so; l] => cf_copyaw8str s so l
+             | _ => cf_bottom)
         | WordFromInt W8 =>
           (case args of
              | [i] => cf_wordFromInt_W8 i
@@ -1804,6 +1826,7 @@ val cf_defs = [
   cf_aw8update_def,
   cf_copyaw8aw8_def,
   cf_copystraw8_def,
+  cf_copyaw8str_def,
   cf_wordFromInt_W8_def,
   cf_wordFromInt_W64_def,
   cf_wordToInt_W8_def,
@@ -2702,6 +2725,31 @@ val cf_sound = Q.store_thm ("cf_sound",
       simp[GSYM o_DEF,n2w_ORD_CHR_w2n] \\
       SPLIT_TAC
     ) \\
+    try_finally (
+      (* CopyAw8Str *)
+      Q.REFINE_EXISTS_TAC `Val v'` \\ simp [] \\ cf_evaluate_step_tac \\
+      GEN_EXISTS_TAC "ck" `st.clock` \\ fs [with_clock_self] \\
+      cf_exp2v_evaluate_tac `st` \\
+      fs [st2heap_def,app_copyaw8str_def] \\
+      fs [W8ARRAY_def] \\
+      fs [SEP_EXISTS, cond_def, SEP_IMP_def, STAR_def, one_def, cell_def] \\
+      first_x_assum progress
+      \\ rename1 `s = Loc ls` \\ rw [] \\
+      assume_tac (GEN_ALL Mem_NOT_IN_ffi2heap) \\
+      (rename1 `W8array _` \\
+        `Mem ls (W8array ws) IN (store2heap st.refs)` by SPLIT_TAC) \\
+      progress store2heap_IN_LENGTH \\ progress store2heap_IN_EL \\
+      fs [do_app_def, store_lookup_def, store_assign_def, store_v_same_type_def, IMPLODE_EXPLODE_I] \\
+      fs[copy_array_def,integerTheory.INT_ABS] \\
+      rpt(full_case_tac THEN1 (irule FALSITY \\ intLib.ARITH_TAC)) \\
+      fs[ws_to_chars_def,chars_to_ws_def] \\
+      fs [evaluateTheory.list_result_def] \\
+      qexists_tac `Mem ls (W8array ws) INSERT u` \\
+      qexists_tac `{}` \\ mp_tac store2heap_IN_unique_key \\ rpt strip_tac
+      THEN1 (progress_then (fs o sing) store2heap_LUPDATE \\ SPLIT_TAC) \\
+      fs[o_DEF] \\
+      first_assum irule \\
+      SPLIT_TAC ) \\
     try_finally (
       (* CopyAw8Aw8 *)
       Q.REFINE_EXISTS_TAC `Val v'` \\ simp [] \\ cf_evaluate_step_tac \\
